Cherry-pick Jay's commit b5db8ae073a92038a32b9432dfd06fa1142c4d3e
Introduce heaplet indices to locations. See msg.

Some of the proofs that we need to write given the introduction of
these indices _may_ need some abstraction breaking. I am not sure if
this _really_ needs to be done, but at least this sets up the stage
for how these locations should look towards client-facing code, so
that may need to be fixed up.

vale/code/arch/Vale.Arch.Heap.fst
@@ -46,3 +46,6 @@ let heap_create_impl ih mt =
     vf_heap = vh;
     vf_heaplets = empty_vale_heaplets vh;
   }
+
+let heap_get_heaplet hi k =
+  (Map16.sel hi.vf_heaplets k).mh
